examples/graph/lib/Data/Graph/Inductive/Internal/Heap.v
@@ -14,6 +14,7 @@ Require Coq.Program.Wf.
 
 Require Import Coq.Lists.List.
 Require Import Lia.
+Require Import PeanoNat.
 Require Import Wellfounded.
 
 (* Converted imports: *)
@@ -39,15 +40,6 @@ Arguments Node {_} {_} _ _ _.
 
 (* Converted value declarations: *)
 
-(* Skipping all instances of class `GHC.Base.Eq_', including
-   `Data.Graph.Inductive.Internal.Heap.Eq___Heap' *)
-
-(* Skipping all instances of class `GHC.Show.Show', including
-   `Data.Graph.Inductive.Internal.Heap.Show__Heap' *)
-
-(* Skipping all instances of class `GHC.Read.Read', including
-   `Data.Graph.Inductive.Internal.Heap.Read__Heap' *)
-
 (* Skipping all instances of class `Control.DeepSeq.NFData', including
    `Data.Graph.Inductive.Internal.Heap.NFData__Heap' *)
 
@@ -55,13 +47,13 @@ Arguments Node {_} {_} _ _ _.
 
 (* Skipping definition `Data.Graph.Inductive.Internal.Heap.printPrettyHeap' *)
 
-Definition empty {a : Type} {b : Type} : Heap a b :=
+#[global] Definition empty {a : Type} {b : Type} : Heap a b :=
   Empty.
 
-Definition unit {a : Type} {b : Type} : a -> b -> Heap a b :=
+#[global] Definition unit {a : Type} {b : Type} : a -> b -> Heap a b :=
   fun key val => Node key val nil.
 
-Definition merge {a : Type} {b : Type} `{GHC.Base.Ord a}
+#[global] Definition merge {a : Type} {b : Type} `{GHC.Base.Ord a}
    : Heap a b -> Heap a b -> Heap a b :=
   fun arg_0__ arg_1__ =>
     match arg_0__, arg_1__ with
@@ -72,7 +64,7 @@ Definition merge {a : Type} {b : Type} `{GHC.Base.Ord a}
         Node key2 val2 (cons h hs')
     end.
 
-Definition insert {a : Type} {b : Type} `{GHC.Base.Ord a}
+#[global] Definition insert {a : Type} {b : Type} `{GHC.Base.Ord a}
    : (a * b)%type -> Heap a b -> Heap a b :=
   fun '(pair key val) => merge (unit key val).
 
@@ -84,17 +76,18 @@ Fixpoint mergeAll {a : Type} {b : Type} `{GHC.Base.Ord a} (arg_0__
      | cons h (cons h' hs) => merge (merge h h') (mergeAll hs)
      end.
 
-Definition isEmpty {a : Type} {b : Type} : Heap a b -> bool :=
+#[global] Definition isEmpty {a : Type} {b : Type} : Heap a b -> bool :=
   fun arg_0__ => match arg_0__ with | Empty => true | _ => false end.
 
-Definition findMin {a} {b} `{HsToCoq.Err.Default (a * b)} : Heap a b -> a * b :=
+#[global] Definition findMin {a} {b} `{HsToCoq.Err.Default (a * b)}
+   : Heap a b -> a * b :=
   fun arg_0__ =>
     match arg_0__ with
     | Empty => GHC.Err.error (GHC.Base.hs_string__ "Heap.findMin: empty heap")
     | Node key val _ => pair key val
     end.
 
-Definition deleteMin {a : Type} {b : Type} `{GHC.Base.Ord a}
+#[global] Definition deleteMin {a : Type} {b : Type} `{GHC.Base.Ord a}
    : Heap a b -> Heap a b :=
   fun arg_0__ =>
     match arg_0__ with
@@ -102,8 +95,10 @@ Definition deleteMin {a : Type} {b : Type} `{GHC.Base.Ord a}
     | Node _ _ hs => mergeAll hs
     end.
 
-Definition splitMin {a} {b} `{GHC.Base.Ord a} `{HsToCoq.Err.Default (a * b *
-                                                                     Heap a b)}
+#[global] Definition splitMin {a} {b} `{GHC.Base.Ord a} `{HsToCoq.Err.Default (a
+                                                                               *
+                                                                               b *
+                                                                               Heap a b)}
    : Heap a b -> a * b * Heap a b :=
   fun arg_0__ =>
     match arg_0__ with
@@ -111,7 +106,7 @@ Definition splitMin {a} {b} `{GHC.Base.Ord a} `{HsToCoq.Err.Default (a * b *
     | Node key val hs => pair (pair key val) (mergeAll hs)
     end.
 
-Definition build {a : Type} {b : Type} `{GHC.Base.Ord a}
+#[global] Definition build {a : Type} {b : Type} `{GHC.Base.Ord a}
    : list (a * b)%type -> Heap a b :=
   Data.Foldable.foldr insert Empty.
 
@@ -142,7 +137,7 @@ Proof.
   - reflexivity.
   - destruct l.
     + simpl. lia.
-    + simpl. repeat(rewrite merge_size). rewrite H1. lia. simpl. lia.
+    + simpl. repeat(rewrite merge_size). rewrite Nat.add_assoc. rewrite H1. reflexivity. simpl. lia.
 Qed.
 
 Lemma deleteMin_size {a} {b} `{GHC.Base.Ord a} (h : Heap a b) : h <> Empty ->
@@ -167,7 +162,8 @@ Program Fixpoint toList {a} {b} `{GHC.Base.Ord a} `{HsToCoq.Err.Default (a * b)}
      end.
 Solve Obligations with ((Tactics.program_simpl; apply toList_termination; auto)).
 
-Definition heapsort {a} `{GHC.Base.Ord a} `{HsToCoq.Err.Default (a * a)}
+#[global] Definition heapsort {a} `{GHC.Base.Ord a} `{HsToCoq.Err.Default (a *
+                                                                           a)}
    : list a -> list a :=
   GHC.Base.map Data.Tuple.fst GHC.Base.∘
   (toList GHC.Base.∘ (build GHC.Base.∘ GHC.Base.map (fun x => pair x x))).
