examples/graph/module-edits/Data/Graph/Inductive/Graph/preamble.v
@@ -1,4 +1,4 @@
-Require Import Omega.
+Require Import Lia.
 Require Import Lists.List.
 Require Import Coq.Sorting.Permutation.
 Require Import Coq.NArith.BinNat.
